Test_Float_Trigonometry.fs
@@ -1,0 +1,12 @@
+module Test_Float_Trigonometry
+
+open Test_Float
+
+let pi: float = System.Single.Pi
+let piHalf: float = System.Single.Pi / 2f
+
+let inline sin (x: float) : float = float.Sin(x / 180f * pi)
+let inline cos (x: float) : float = float.Cos(x / 180f * pi)
+let inline sinCos (x: float) : struct (float * float) = float.SinCos(x / 180f * pi)
+let inline arctg (x: float) (y: float) : float = float.Atan2(y, x) * 180f / pi
+let inline hypot (x: float) (y: float) : float = float.Hypot(x, y)
