Test.Float.fsti
@@ -13,14 +13,58 @@ let float_extension : extension_parser = fun s ->
   | 'f'::tl -> Some (extension, tl)
   | _ -> None
 
-type mantType = int
-type powerType = e: int{e <= 0}
-type mant_pow' = mantType & powerType
-type mant_pow = x: mant_pow'{x._1 % 10 = 0 ==> x._2 = 0}
+type mant_pow' = int & int
+type mant_pow = x: mant_pow'{x._1 % 10 = 0 ==> (x._1 = 0 /\ x._2 = 0)}
+
+let rec pow10 (x: nat) : GTot pos =
+  match x with
+  | 0 -> 1
+  | _ -> 10 * pow10 (x - 1)
+let rec norm_pair (mp: mant_pow') : Tot mant_pow (decreases abs (fst mp)) =
+  let mantissa = fst mp in
+  let power = snd mp in
+  if mantissa = 0
+  then 0, 0
+  else if mantissa % 10 = 0
+       then norm_pair (mantissa / 10, power + 1)
+       else mp
+
+let rec lemma_norm_pow_add (n: int) (mp': mant_pow') (mp_': mant_pow') : Lemma 
+  (requires fst mp' <> 0 /\ mp_' = (fst mp', snd mp' + n))
+  (ensures (let mp = norm_pair mp' in norm_pair mp_' = (fst mp, snd mp + n)))
+  (decreases abs (fst mp'))
+  =
+  match fst mp' % 10 with
+  | 0 -> 
+    let mp'' = (fst mp' / 10, snd mp' + 1) in
+    let mp_'' = (fst mp_' / 10, snd mp_' + 1) in
+    lemma_norm_pow_add n mp'' mp_''
+  | _ -> ()
+
+let rec lemma_norm_mant_mul' (n: nat) (mp: mant_pow) : Lemma 
+  (requires fst mp <> 0)
+  (ensures norm_pair (fst mp * pow10 n, snd mp) = (fst mp, snd mp + n))
+  =
+  match n with
+  | 0 -> ()
+  | _ ->
+    lemma_norm_mant_mul' (n - 1) mp;
+    let mant', pow' = fst mp * pow10 (n - 1), snd mp + n - 1 in
+    assert (norm_pair (mant', snd mp) = (fst mp, pow'));
+    lemma_norm_pow_add 1 (mant', snd mp) (mant', snd mp + 1);
+    assert (norm_pair (mant', snd mp + 1) = (fst mp, pow' + 1));
+    assert (norm_pair (mant' * 10, snd mp) = norm_pair (mant', snd mp + 1));
+    assert (norm_pair (mant' * 10, snd mp) = (fst mp, pow' + 1))
+
+let lemma_norm_mant_mul (n: nat) (mant: int) (pow: int) : Lemma
+  (requires mant % 10 <> 0)
+  (ensures norm_pair (mant * pow10 n, pow) = (mant, pow + n))
+  [SMTPat (norm_pair (mant * pow10 n, pow))]
+  = lemma_norm_mant_mul' n (mant, pow)
 
 val to_pair (x: float) : mant_pow
 val of_pair (mant_power: mant_pow) : float
-let of_int (x: int) : float = of_pair (x, 0)
+let of_int (x: int) : float = of_pair (norm_pair (x, 0))
 
 val lemma_of_to_inv (x: float) : Lemma (of_pair (to_pair x) = x) [SMTPat (to_pair x)]
 val lemma_to_of_inv (x: mant_pow) : Lemma (to_pair (of_pair x) = x) [SMTPat (of_pair x)]
@@ -28,26 +72,11 @@ val lemma_to_of_inv (x: mant_pow) : Lemma (to_pair (of_pair x) = x) [SMTPat (of_
 val zero : (z: float{z = of_pair (0, 0)})
 val one : (o: float{o = of_pair (1, 0)})
 
+
 type not_zero = (nz: float{nz <> zero})
 
-let mantissa (x: float) : GTot mantType = (to_pair x)._1
-let power (x: float) : GTot powerType = (to_pair x)._2
-
-
-let rec pow10 (x: nat) : GTot pos =
-  match x with
-  | 0 -> 1
-  | _ -> 10 * pow10 (x - 1)
-let rec incr_power (mp: mant_pow') : GTot (x: mant_pow'{x._1 % 10 = 0 ==> x._2 = 0}) (decreases (-mp._2)) =
-    if mp._1 % 10 = 0 && mp._2 < 0
-    then incr_power (mp._1 / 10, mp._2 + 1)
-    else mp
-let norm_pair (mant_pow: mant_pow') : GTot (x: mant_pow'{x._1 % 10 = 0 ==> x._2 = 0}) =
-  let mantissa = mant_pow._1 in
-  let exp = mant_pow._2 in
-  match mantissa with
-  | 0 -> 0, 0
-  | _ -> incr_power mant_pow
+let mantissa (x: float) : GTot int = (to_pair x)._1
+let power (x: float) : GTot int = (to_pair x)._2
 
 
 val add (a b: float) : Pure float
@@ -58,7 +87,7 @@ val add (a b: float) : Pure float
     let pow_min = min pow_a pow_b in
     let a' = (mantissa a) * pow10 (pow_a - pow_min) in
     let b' = (mantissa b) * pow10 (pow_b - pow_min) in
-    to_pair c = (a' + b', pow_min))
+    to_pair c = norm_pair (a' + b', pow_min))
 
 val sub (a b: float) : Pure float
   (requires True)
@@ -66,9 +95,9 @@ val sub (a b: float) : Pure float
     let mant_a, pow_a = to_pair a in
     let mant_b, pow_b = to_pair b in
     let pow_min = min pow_a pow_b in
-    let a' = (mantissa a) * pow10 (pow_a - pow_min) in
-    let b' = (mantissa b) * pow10 (pow_b - pow_min) in
-    to_pair c = (a' - b', pow_min))
+    let a' = mant_a * pow10 (pow_a - pow_min) in
+    let b' = mant_b * pow10 (pow_b - pow_min) in
+    to_pair c = norm_pair (a' - b', pow_min))
 
 val neg (a: float) : Pure float
   (requires True)
@@ -78,12 +107,22 @@ val mul (a b: float) : Pure float
   (requires True)
   (ensures fun c -> to_pair c = norm_pair (mantissa a * mantissa b, power a + power b))
 
-val div (a: float) (b: not_zero) : float
+val div (a: float) (b: not_zero) : Pure float
+  (requires True)
+  (ensures fun c -> c `mul` b = a)
+
+val inv (a: not_zero) : Pure not_zero
+  (requires True)
+  (ensures fun b -> b = one `div` a)
 
 val gt (a b: float) : Pure bool (requires True) (ensures fun c -> c <==> mantissa (a `sub` b) > 0)
 val lt (a b: float) : Pure bool (requires True) (ensures fun c -> c <==> mantissa (a `sub` b) < 0)
 val gte (a b: float) : Pure bool (requires True) (ensures fun c -> c <==> mantissa (a `sub` b) >= 0)
 val lte (a b: float) : Pure bool (requires True) (ensures fun c -> c <==> mantissa (a `sub` b) <= 0)
+
+val abs (a: float) : Pure float
+  (requires True)
+  (ensures fun b -> if a `lt` zero then b = neg a else b = a)
 
 unfold let ( +. ) a b = add a b
 unfold let ( -. ) a b = sub a b
@@ -96,62 +135,49 @@ unfold let (<.) a b = lt a b
 unfold let (>=.) a b = gte a b
 unfold let (<=.) a b = lte a b
 
-
-val abs (a: float) : Pure float
-  (requires True)
-  (ensures fun b -> (if a <. zero then b = ~.a else b = a) /\ b >=. zero)
-
 let lemma_commut_add a b : Lemma (a +. b = b +. a) = ()
 let lemma_commut_mul a b : Lemma (a *. b = b *. a) = ()
 
-let lemma_add_zero a : Lemma (a +. zero = a) = ()
+let lemma_add_zero (a: float) : Lemma (a `add` zero = a) = ()
 let lemma_mul_one  a : Lemma (a *. one  = a) = ()
 let lemma_mul_zero a : Lemma (a *. zero = zero) = ()
+let lemma_div_one  a : Lemma (a /. one = a) = ()
 
-let lemma_sub_neg a : Lemma (~.a = zero -. a) = ()
+let test () = assert (zero = of_pair (0, 0))
+
+let lemma_sub_neg (a: float) : Lemma (~.a = zero -. a) =
+  match a = zero with
+  | true -> ()
+  | _ -> 
+    let mant_z, pow_z = to_pair zero in
+    let mant_a, pow_a = to_pair a in
+    let pow_min = min pow_a pow_z in
+    let z' = mant_z * pow10 (pow_z - pow_min) in
+    let a' = mant_a * pow10 (pow_a - pow_min) in
+    match pow_min with
+    | 0 ->
+      assert (z' - a' = - mant_a * pow10 pow_a);
+      lemma_norm_mant_mul pow_a (-mant_a) pow_min
+    | _ -> ()
+  
 let lemma_neg_neg a : Lemma (~.(~.a) = a) = ()
 let lemma_add_neg a : Lemma (a -. a = zero) = ()
+let lemma_sub_add a b : Lemma (a -. b = a +. ~.b) = ()
+// let lemma_div_inv a : Lemma (a /. a = one) = ()
+// let lemma_inv_inv a : Lemma (inv (inv a) = a) = ()
 
 let lemma_additive_add_left a b c : Lemma (a +. b +. c = (a +. b) +. c) = ()
 let lemma_additive_add_right a b c : Lemma (a +. b +. c = a +. (b +. c)) [SMTPat (a +. b +. c)] =
   assume (a +. b +. c = a +. (b +. c))
+let lemma_additive_sub_right a b c : Lemma (a +. b -. c = a +. (b -. c)) [SMTPat (a +. b -. c)] =
+  assume (a +. b -. c = a +. (b -. c))
 let lemma_additive_mul_left a b c : Lemma (a *. b *. c = (a *. b) *. c) = ()
-let lemma_additive_mul_right a b c : Lemma (a *. b *. c = a *. (b *. c)) = 
+let lemma_additive_mul_right a b c : Lemma (a *. b *. c = a *. (b *. c)) [SMTPat (a *. b *. c)] = 
   assume (a *. b *. c = a *. (b *. c))
 
 let lemma_add_perenos a b c : Lemma (requires a +. b = c) (ensures a = c -. b) =
   assert (a +. b -. b = c -. b);
-  lemma_additive_add_right a b (~.b)
+  lemma_additive_sub_right a b b
 
-let lemma_distrib_add a b c : Lemma (a *. (b +. c) = a *. b +. a *. c) = assume (a *. (b +. c) = a *. b +. a *. c)
-
-// let lemma_gt a b : Lemma (requires a >. b) (ensures a -. b >. zero) = ()
-
-
-let ( .[] ) x (min, max) = min <=. x && x <=. max
-let ( .() ) x (min, max) = min <. x && x <. max
-let ( <.|> ) x (min, max) = min <=. x && x <. max
-let ( <|.> ) x (min, max) = min <. x && x <=. max
-
-let pi : float = of_int 180
-let piHalf : float = of_int 90
-
-val sin : float -> (r: float{r.[~.one, one]})
-val cos : float -> (r: float{r.[~.one, one]})
-val arctg (x y: float) : (r: float{r.[~.pi, pi]})
-val hypot (x y: float) : (r: float{r *. r = x *. x +. y *. y /\ r >=. zero})
-
-val lemma_sin_odd  (a: float) : Lemma (sin a = ~.(sin ~.a))
-val lemma_cos_even (a: float) : Lemma (cos a = cos ~.a)
-val lemma_arctg_x_pos x y : Lemma (requires x >=. zero) (ensures (arctg x y).(~.piHalf, piHalf)) [SMTPat (arctg x y)]
-
-val lemma_sin_0 (a: float{a = zero}) : Lemma (sin a = zero)
-val lemma_cos_0 (a: float{a = zero}) : Lemma (cos a = one)
-let lemma_sin_cos_0 (a: float{a = zero}) : Lemma (sin a = zero /\ cos a = one) = lemma_sin_0 a; lemma_cos_0 a
-
-val lemma_sin_90 (a: float{a = of_int 90}) : Lemma (sin a = one)
-val lemma_cos_90 (a: float{a = of_int 90}) : Lemma (cos a = zero)
-let lemma_sin_cos_90 (a: float{a = of_int 90}) : Lemma (sin a = one /\ cos a = zero) = lemma_sin_90 a; lemma_cos_90 a
-
-val lemma_cos_add (a b: float) : Lemma (cos (a +. b) = cos a *. cos b -. sin a *. sin b)
-val lemma_sin_add (a b: float) : Lemma (sin (a +. b) = sin a *. cos b +. cos a *. sin b)
+let lemma_distrib_add a b c : Lemma (a *. (b +. c) = a *. b +. a *. c) =
+  assume (a *. (b +. c) = a *. b +. a *. c)
