Test.Float.Trigonometry.fsti
@@ -1,0 +1,33 @@
+module Test.Float.Trigonometry
+
+open Test.Float
+
+let ( .[] ) x (min, max)  = min <=. x && x <=. max
+let ( .() ) x (min, max)  = min <. x && x <. max
+let ( <.|> ) x (min, max) = min <=. x && x <. max
+let ( <|.> ) x (min, max) = min <. x && x <=. max
+
+let pi : float = of_int 180
+let piHalf : float = of_int 90
+
+val sin : float -> (r: float{r.[~.one, one]})
+val cos : float -> (r: float{r.[~.one, one]})
+val arctg (x y: float) : (r: float{r.[~.pi, pi]})
+val hypot (x y: float) : (r: float{r *. r = x *. x +. y *. y /\ r >=. zero})
+
+val lemma_sin_odd  (a: float) : Lemma (sin a = ~.(sin ~.a))
+val lemma_cos_even (a: float) : Lemma (cos a = cos ~.a)
+val lemma_arctg_x_pos x y : Lemma (requires x >=. zero) (ensures (arctg x y).(~.piHalf, piHalf)) [SMTPat (arctg x y)]
+
+val lemma_sin_0 (a: float{a = zero}) : Lemma (sin a = zero)
+val lemma_cos_0 (a: float{a = zero}) : Lemma (cos a = one)
+let lemma_sin_cos_0 (a: float{a = zero}) : Lemma (sin a = zero /\ cos a = one) = lemma_sin_0 a; lemma_cos_0 a
+
+val lemma_sin_90 (a: float{a = of_int 90}) : Lemma (sin a = one)
+val lemma_cos_90 (a: float{a = of_int 90}) : Lemma (cos a = zero)
+let lemma_sin_cos_90 (a: float{a = of_int 90}) : Lemma (sin a = one /\ cos a = zero) = lemma_sin_90 a; lemma_cos_90 a
+
+val lemma_cos_add (a b: float) : Lemma (cos (a +. b) = cos a *. cos b -. sin a *. sin b)
+val lemma_sin_add (a b: float) : Lemma (sin (a +. b) = sin a *. cos b +. cos a *. sin b)
+
+val lemma_arctg (a: float{a.[~.pi, pi]}) : Lemma (arctg (cos a) (sin a) = a)
