Test.Program.fst
@@ -8,9 +8,8 @@ open Test.Float
 let main =
   let x = of_pair (2, -1) in
   let y = of_pair (4, 0) in
-  let z = x -. one in
-  assert (zero >=. zero);
-  assert (x -. y = ~. y +. x);
+  let z = x +. y in
+  assert (z = of_pair (42, -1));
 
   let msg = Printf.ext_sprintf float_extension
     "%Xf * %Xf = %Xf\n"
